Proof done

Project.v
@@ -510,12 +510,11 @@ Inductive insert_kind : nat -> env -> env -> Prop :=
 | insert_0 : forall k e,
                    insert_kind 0 e (v_typ k e)
 | insert_S_v : forall n tp e e',
-               insert_kind (S n) e e' ->
+               insert_kind (S n) e e' -> wf_typ e' (tshift tp n) ->
                insert_kind (S n) (v tp e) (v (tshift tp n) e')
 | insert_S_v_typ : forall n k e e',
                    insert_kind n e e' ->
-                   insert_kind (S n) e (v_typ k e')
-.
+                   insert_kind (S n) e (v_typ k e').
 
 Lemma wf_env_typ : forall e tp, wf_env (v tp e) -> wf_typ e tp.
 Proof.
@@ -530,13 +529,29 @@ Lemma insert_kind_wf_typ : forall (X : nat) (e e' : env) (tp : typ),
                              wf_env (v (tshift tp X) e').
 Proof.
 *)
-Lemma insert_kind_wf_env : forall (X : nat) (e e' : env),
+
+
+Lemma insert_kind_wf_env : forall (e':env) (X:nat) (e:env),
                              insert_kind X e e' -> wf_env e -> wf_env e'.
-induction X; intros e e' H wfness.
-+ inversion H.
-  easy.
-+ destruct e'; inversion H; simpl.
-  - now apply (IHX e).
-  - split.
-    * apply wf_env_typ.
-      apply insert_kind_wf_env.
+induction e'; intros X  e kd wf.
+- easy.
+- induction e;inversion kd.
+  + easy.
+  + apply (IHe' n0 empty); easy.
+  + easy.
+  + apply (IHe' n1 (v_typ n0 e)); easy.
+  + easy.
+  + apply (IHe' n0 (v t e)); easy.
+- induction e; inversion kd. 
+  * simpl.
+    split.
+    apply H5.
+    apply (IHe' X e).
+    rewrite <- H1.
+    apply H3.
+    simpl in wf.
+    destruct wf.
+    apply H7.
+Qed.
+    
+    
